change formula_def, include basic proof

BBI.thy
@@ -13,24 +13,55 @@ section "BBI formula"
 (* We define a variable which is indexed by natural number. In this way we can genereate inifinte atomic proposition varaiables *)
 datatype atom = P nat
 
+(* We now define a axiom which can evaluate atom to boolean *)
+axiomatization evalP :: "atom \<Rightarrow> bool" 
+
 (* With inifinte proposition variablse we can now define BBI formula. N.B. Capial M means the connective is a multiplicative connective *)
-datatype BBI_form = Atom atom
-  | Neg  BBI_form  
-  | Mneg BBI_form 
-  | Con BBI_form BBI_form
-  | MCon BBI_form BBI_form
-  | Dis BBI_form BBI_form
-  | Mdis BBI_form BBI_form
+datatype BBI_form = 
+  Truth                     ("\<top>\<^sub>B")
+  | Falsity                 ("\<bottom>\<^sub>B")
+  | Atom atom
+  | Neg  BBI_form           ("\<not>\<^sub>B _" 100)
+  | Mneg BBI_form           ("~\<^sub>B _" 100)
+  | Con BBI_form BBI_form   (infix "\<and>\<^sub>B" 101)
+  | MCon BBI_form BBI_form  (infix "*\<^sub>B" 101)
+  | Dis BBI_form BBI_form   (infix "\<or>\<^sub>B" 101)
+  | Mdis BBI_form BBI_form  (infix "\<or>*\<^sub>B" 101)
 
-(* We now define a constant  which can evaluate BBI_form to Boolean type but we dont define how it is done*)
-consts evalF :: "BBI_form \<Rightarrow> bool" 
+(* We now define a recursive evaluation to evaluate BBI formula to a boolean type*)
+primrec evalF :: "BBI_form \<Rightarrow> bool" where
+  "evalF Truth = True"|
+  "evalF Falsity = False"|
+  "evalF (Atom p) = evalP p"|
+  "evalF (\<not>\<^sub>B \<phi>) = (\<not>(evalF \<phi>))"|
+  "evalF (~\<^sub>B \<phi>) =  (\<not>(evalF \<phi>))" |
+  "evalF (\<phi> \<and>\<^sub>B \<psi>) = ((evalF \<phi> )\<and>(evalF \<psi>))"|
+  "evalF (\<phi> *\<^sub>B \<psi>) = ((evalF \<phi> )\<and>(evalF \<psi>))"|
+  "evalF (\<phi> \<or>\<^sub>B \<psi>) = ((evalF \<phi> )\<or>(evalF \<psi>))"|
+  "evalF (\<phi> \<or>*\<^sub>B \<psi>) = ((evalF \<phi> )\<or>(evalF \<psi>))"
 
-(* An automatic induction proof for any BBI formula you can induct the next BBI formula *)
-lemma BBI_induc: "BBI_form \<Longrightarrow> BBI_form"
-proof auto
-qed
+definition "evaluation \<phi> \<equiv>  {\<xi>. \<xi>(evalF \<phi>)}"
+
+(* Here we have to create a lemma to show that negation of atomic BBI formula is equal to the negation of atomic proposition*)
+lemma negateAtom : 
+  "evalF (Neg (Atom a)) \<Longrightarrow>  \<not>(evalP a)" 
+  "evalF (Mneg (Atom a)) \<Longrightarrow>  \<not>(evalP a)"
+  "evalF (Neg Truth) \<Longrightarrow>  False" 
+  "evalF (Neg Falsity) \<Longrightarrow>  True" 
+  "evalF (Mneg Truth) \<Longrightarrow>  False" 
+  "evalF (Mneg Falsity) \<Longrightarrow> True" 
+  by auto
+
+(* Basic Axiom for both CL and LM using auto proof through induction*)
+lemma Ax : "evalF f \<Longrightarrow> evalF f"
+  by auto
+
+section "Classical Logic Axioms and Rules"
+
+lemma top: "evalF f \<Longrightarrow> True"
+  by auto
+
+lemma bot: "False \<Longrightarrow> evalF f"
+  by auto
 
 
-
-
-end
